thys/MRBNF_Recursor.thy
@@ -126,7 +126,4 @@ lemma supp_if: "|supp (u::'a \<Rightarrow> 'a)| <o |UNIV::'a set| \<Longrightarr
 lemma imsupp_if_empty: "imsupp u \<inter> A = {} \<Longrightarrow> imsupp (if P then id else u) \<inter> A = {}" unfolding imsupp_def supp_def by simp
 lemma image_if_empty: "u ` A \<inter> B = {} \<Longrightarrow> (P \<Longrightarrow> A \<inter> B = {}) \<Longrightarrow> (if P then id else u) ` A \<inter> B = {}" by simp
 
-ML_file \<open>../Tools/mrbnf_recursor_tactics.ML\<close>
-ML_file \<open>../Tools/mrbnf_recursor.ML\<close>
-
 end
